fstar/MLS.TreeSync.API.fst
@@ -6,24 +6,31 @@ open MLS.NetworkTypes
 open MLS.TreeSync.NetworkTypes
 open MLS.Tree
 open MLS.TreeCommon
+open MLS.TreeSync.Types
 open MLS.TreeSync.Operations
 open MLS.TreeSync.Refined.Types
 open MLS.TreeSync.Refined.Operations
 open MLS.TreeSync.API.Types
 open MLS.Result
 
-#set-options "--fuel 1 --ifuel 1"
+#set-options "--fuel 0 --ifuel 0"
 
-val create: #bytes:Type0 -> {|crypto_bytes bytes|} -> #tkt:treekem_types bytes -> gid:mls_bytes bytes -> leaf_node_nt bytes tkt -> treesync_state bytes tkt
-let create #bytes #cb gid lp =
-  {
-    group_id = gid;
-    levels = 0;
-    tree = create_tree lp;
-    version = 0;
-  }
+#push-options "--fuel 1 --ifuel 1"
+val create: #bytes:Type0 -> {|crypto_bytes bytes|} -> #tkt:treekem_types bytes -> group_id:mls_bytes bytes -> ln:leaf_node_nt bytes tkt -> result (treesync_state bytes tkt)
+let create #bytes #cb group_id ln =
+  if not (leaf_is_valid group_id ln) then
+    error "create: leaf node is not valid"
+  else (
+    return ({
+      group_id;
+      levels = 0;
+      tree = create_tree ln;
+      version = 0;
+    })
+  )
+#pop-options
 
-val state_update_tree: #bytes:Type0 -> {|crypto_bytes bytes|} -> #tkt:treekem_types bytes -> #l:nat -> treesync_state bytes tkt -> treesync bytes tkt l 0 -> treesync_state bytes tkt
+val state_update_tree: #bytes:Type0 -> {|crypto_bytes bytes|} -> #tkt:treekem_types bytes -> #l:nat -> st:treesync_state bytes tkt -> treesync_valid bytes tkt l 0 st.group_id -> treesync_state bytes tkt
 let state_update_tree #bytes #cb #tkt #l st new_tree =
   ({ st with
     levels = l;
@@ -42,25 +49,38 @@ let get_leaf_package_from_key_package #bytes #cb kp =
 
 val add: #bytes:Type0 -> {|crypto_bytes bytes|} -> #tkt:treekem_types bytes -> treesync_state bytes tkt -> key_package_nt bytes tkt -> result (treesync_state bytes tkt & nat)
 let add #bytes #cb #tkt st kp =
-  lp <-- get_leaf_package_from_key_package kp;
-  match find_empty_leaf st.tree with
-  | Some i ->
-    if not (tree_add_pre st.tree i) then
-      error "add: tree_add_pre is false"
-    else
-      return (state_update_tree st (tree_add st.tree i lp), (i <: nat))
-  | None ->
-    let extended_tree = tree_extend st.tree in
-    let i = Some?.v (find_empty_leaf extended_tree) in
-    if not (tree_add_pre extended_tree i) then
-      error "add: tree_add_pre is false (after extension)"
-    else
-      return (state_update_tree st (tree_add extended_tree i lp), (i <: nat))
+  ln <-- get_leaf_package_from_key_package kp;
+  if not (ln.data.source = LNS_key_package()) then
+    error "add: bad leaf node source"
+  else if not (leaf_is_valid st.group_id ln) then
+    error "add: invalid leaf node"
+  else (
+    match find_empty_leaf st.tree with
+    | Some i ->
+      if not (tree_add_pre st.tree i) then
+        error "add: tree_add_pre is false"
+      else
+        return (state_update_tree st (tree_add st.tree i ln), (i <: nat))
+    | None ->
+      let extended_tree = tree_extend st.tree in
+      let i = Some?.v (find_empty_leaf extended_tree) in
+      if not (tree_add_pre extended_tree i) then
+        error "add: tree_add_pre is false (after extension)"
+      else
+        return (state_update_tree st (tree_add extended_tree i ln), (i <: nat))
+  )
 
-val update: #bytes:Type0 -> {|crypto_bytes bytes|} -> #tkt:treekem_types bytes -> st:treesync_state bytes tkt -> leaf_node_nt bytes tkt -> treesync_index st -> treesync_state bytes tkt
-let update #bytes #cb #tkt st lp i =
-  state_update_tree st (tree_update st.tree i lp)
+val update: #bytes:Type0 -> {|crypto_bytes bytes|} -> #tkt:treekem_types bytes -> st:treesync_state bytes tkt -> leaf_node_nt bytes tkt -> treesync_index st -> result (treesync_state bytes tkt)
+let update #bytes #cb #tkt st ln i =
+  if not (ln.data.source = LNS_update()) then
+    error "update: leaf node has invalid source"
+  else if not (leaf_is_valid st.group_id ln) then
+    error "update: leaf node is not valid"
+  else (
+    return (state_update_tree st (tree_update st.tree i ln))
+  )
 
+#push-options "--fuel 0 --ifuel 1"
 val remove: #bytes:Type0 -> {|crypto_bytes bytes|} -> #tkt:treekem_types bytes -> st:treesync_state bytes tkt -> i:treesync_index st -> treesync_state bytes tkt
 let remove #bytes #cb #tkt st i =
   let blanked_tree = (tree_remove st.tree i) in
@@ -68,14 +88,13 @@ let remove #bytes #cb #tkt st i =
     state_update_tree st (tree_truncate blanked_tree)
   else
     state_update_tree st blanked_tree
+#pop-options
 
 val commit: #bytes:Type0 -> {|crypto_bytes bytes|} -> #tkt:treekem_types bytes -> st:treesync_state bytes tkt -> #li:treesync_index st -> external_pathsync bytes tkt st.levels 0 li -> result (treesync_state bytes tkt)
 let commit #bytes #cb #tkt st #li p =
   if not (apply_external_path_pre st.tree p) then
     error "commit: bad precondition"
-  else if not (external_path_is_parent_hash_valid st.tree p) then
-    error "commit: bad parent hash"
-  else if not (external_path_is_filter_valid st.tree p) then
-    internal_failure "commit: bad filtering"
+  else if not (external_path_is_valid st.group_id st.tree p) then
+    error "commit: invalid path"
   else
     return (state_update_tree st (apply_external_path st.tree p))
