fstar/MLS.TreeSync.Refined.Operations.fst
@@ -6,60 +6,67 @@ open MLS.NetworkTypes
 open MLS.TreeSync.NetworkTypes
 open MLS.Tree
 open MLS.TreeCommon
+open MLS.TreeSync.Types
 open MLS.TreeSync.Operations
 open MLS.TreeSync.Invariants.UnmergedLeaves.Proofs
 open MLS.TreeSync.Invariants.ParentHash.Proofs
+open MLS.TreeSync.Invariants.ValidLeaves.Proofs
 open MLS.TreeSync.Refined.Types
 
-val tree_add_pre: #bytes:Type0 -> {|crypto_bytes bytes|} -> #tkt:treekem_types bytes -> #l:nat -> #i:tree_index l -> treesync bytes tkt l i -> li:leaf_index l i -> bool
-let tree_add_pre #bytes #cb #tkt #l #i t li = tree_add_pre t li
+#push-options "--fuel 0 --ifuel 0"
 
-val tree_add: #bytes:Type0 -> {|crypto_bytes bytes|} -> #tkt:treekem_types bytes -> #l:nat -> #i:tree_index l -> t:treesync bytes tkt l i -> li:leaf_index l i{leaf_at t li == None} -> leaf_node_nt bytes tkt -> Pure (treesync bytes tkt l i)
-  (requires tree_add_pre t li)
+val tree_add: #bytes:Type0 -> {|crypto_bytes bytes|} -> #tkt:treekem_types bytes -> #l:nat -> #i:tree_index l -> #group_id:mls_bytes bytes -> t:treesync_valid bytes tkt l i group_id -> li:leaf_index l i -> ln:leaf_node_nt bytes tkt -> Pure (treesync_valid bytes tkt l i group_id)
+  (requires leaf_at t li == None /\ ln.data.source == LNS_key_package() /\ leaf_is_valid group_id ln /\ tree_add_pre t li)
   (ensures fun _ -> True)
-let tree_add #bytes #cb #tkt #l #i t li ln =
+let tree_add #bytes #cb #tkt #l #i #group_id t li ln =
   unmerged_leaves_ok_tree_add t li ln;
   parent_hash_invariant_tree_add t li ln;
+  valid_leaves_invariant_tree_add group_id t li ln;
   tree_add t li ln
 
-val tree_update: #bytes:Type0 -> {|crypto_bytes bytes|} -> #tkt:treekem_types bytes -> #l:nat -> #i:tree_index l -> t:treesync bytes tkt l i -> li:leaf_index l i -> leaf_node_nt bytes tkt -> treesync bytes tkt l i
-let tree_update #bytes #cb #tkt #l #i t li ln =
+val tree_update: #bytes:Type0 -> {|crypto_bytes bytes|} -> #tkt:treekem_types bytes -> #l:nat -> #i:tree_index l -> #group_id:mls_bytes bytes -> t:treesync_valid bytes tkt l i group_id -> li:leaf_index l i -> ln:leaf_node_nt bytes tkt -> Pure (treesync_valid bytes tkt l i group_id)
+  (requires ln.data.source == LNS_update() /\ leaf_is_valid group_id ln)
+  (ensures fun _ -> True)
+let tree_update #bytes #cb #tkt #l #i #group_id t li ln =
   unmerged_leaves_ok_tree_update t li ln;
   parent_hash_invariant_tree_update t li ln;
+  valid_leaves_invariant_tree_update group_id t li ln;
   tree_update t li ln
 
-val tree_remove: #bytes:Type0 -> {|crypto_bytes bytes|} -> #tkt:treekem_types bytes -> #l:nat -> #i:tree_index l -> t:treesync bytes tkt l i -> li:leaf_index l i -> treesync bytes tkt l i
-let tree_remove #bytes #cb #tkt #l #i t li =
+val tree_remove: #bytes:Type0 -> {|crypto_bytes bytes|} -> #tkt:treekem_types bytes -> #l:nat -> #i:tree_index l -> #group_id:mls_bytes bytes -> t:treesync_valid bytes tkt l i group_id -> li:leaf_index l i -> treesync_valid bytes tkt l i group_id
+let tree_remove #bytes #cb #tkt #l #i #group_id t li =
   unmerged_leaves_ok_tree_remove t li;
   parent_hash_invariant_tree_remove t li;
+  valid_leaves_invariant_tree_remove group_id t li;
   tree_remove t li
 
-val apply_external_path_pre: #bytes:Type0 -> {|crypto_bytes bytes|} -> #tkt:treekem_types bytes -> #l:nat -> #li:leaf_index l 0 -> t:treesync bytes tkt l 0 -> external_pathsync bytes tkt l 0 li -> bool
-let apply_external_path_pre #bytes #cb #tkt #l #li t p =
-  apply_external_path_pre t p
-
-val apply_external_path: #bytes:Type0 -> {|crypto_bytes bytes|} -> #tkt:treekem_types bytes -> #l:nat -> #li:leaf_index l 0 -> t:treesync bytes tkt l 0 -> p:external_pathsync bytes tkt l 0 li -> Pure (treesync bytes tkt l 0)
-  (requires apply_external_path_pre t p /\ external_path_is_parent_hash_valid t p /\ external_path_is_filter_valid t p)
+#push-options "--ifuel 1"
+val apply_external_path: #bytes:Type0 -> {|crypto_bytes bytes|} -> #tkt:treekem_types bytes -> #l:nat -> #li:leaf_index l 0 -> #group_id:mls_bytes bytes -> t:treesync_valid bytes tkt l 0 group_id -> p:external_pathsync bytes tkt l 0 li -> Pure (treesync_valid bytes tkt l 0 group_id)
+  (requires apply_external_path_pre t p /\ external_path_is_valid group_id t p)
   (ensures fun _ -> True)
-let apply_external_path #bytes #cb #tkt #l #li t p =
+let apply_external_path #bytes #cb #tkt #l #li #group_id t p =
   unmerged_leaves_ok_apply_external_path t p;
   parent_hash_invariant_apply_external_path t p;
+  valid_leaves_invariant_apply_external_path group_id t p;
   apply_external_path t p
+#pop-options
 
-val mk_blank_tree: #bytes:Type0 -> {|crypto_bytes bytes|} -> #tkt:treekem_types bytes -> l:nat -> i:tree_index l -> treesync bytes tkt l i
-let mk_blank_tree #bytes #cb #tkt l i =
-  unmerged_leaves_ok_mk_blank_tree #bytes #cb.base #tkt l i;
-  parent_hash_invariant_mk_blank_tree #bytes #cb #tkt l i;
-  mk_blank_tree l i
-
-val tree_extend: #bytes:Type0 -> {|crypto_bytes bytes|} -> #tkt:treekem_types bytes -> #l:nat -> t:treesync bytes tkt l 0 -> treesync bytes tkt (l+1) 0
-let tree_extend #bytes #cb #tkt #l t =
+#push-options "--ifuel 1"
+val tree_extend: #bytes:Type0 -> {|crypto_bytes bytes|} -> #tkt:treekem_types bytes -> #l:nat -> #group_id:mls_bytes bytes -> t:treesync_valid bytes tkt l 0 group_id -> treesync_valid bytes tkt (l+1) 0 group_id
+let tree_extend #bytes #cb #tkt #l #group_id t =
   unmerged_leaves_ok_tree_extend t;
   parent_hash_invariant_tree_extend t;
+  valid_leaves_invariant_tree_extend group_id t;
   tree_extend t
+#pop-options
 
-val tree_truncate: #bytes:Type0 -> {|crypto_bytes bytes|} -> #tkt:treekem_types bytes -> #l:pos -> t:treesync bytes tkt l 0{is_tree_empty (TNode?.right t)} -> treesync bytes tkt (l-1) 0
-let tree_truncate #bytes #cb #tkt #l t =
+#push-options "--ifuel 1"
+val tree_truncate: #bytes:Type0 -> {|crypto_bytes bytes|} -> #tkt:treekem_types bytes -> #l:pos -> #group_id:mls_bytes bytes -> t:treesync_valid bytes tkt l 0 group_id -> Pure (treesync_valid bytes tkt (l-1) 0 group_id)
+  (requires is_tree_empty (TNode?.right t))
+  (ensures fun _ -> True)
+let tree_truncate #bytes #cb #tkt #l #group_id t =
   unmerged_leaves_ok_tree_truncate t;
   parent_hash_invariant_tree_truncate t;
+  valid_leaves_invariant_tree_truncate group_id t;
   tree_truncate t
+#pop-options
